intermediate/Veritas.Intermediate.StoreS.fst
@@ -1,0 +1,97 @@
+module Veritas.Intermediate.StoreS
+
+let get_slot (st:vstore) (s:slot_id)
+  : option vstore_entry
+  = if s >= Seq.length st then None 
+    else Seq.index st s
+
+let store_contains (st:vstore) (s:slot_id) : bool
+  = Some? (get_slot st s)
+
+let stored_key (st:vstore) (s:slot_id{store_contains st s}) : key
+  = VStoreE?.k (Some?.v (get_slot st s))
+
+let stored_value (st:vstore) (s:slot_id{store_contains st s}) : value
+  = VStoreE?.v (Some?.v (get_slot st s))
+
+let add_method_of (st:vstore) (s:slot_id{store_contains st s}) : add_method
+  = VStoreE?.am (Some?.v (get_slot st s))
+
+let l_child_in_store (st:vstore) (s:slot_id{store_contains st s}) : bool
+  = VStoreE?.l_child_in_store (Some?.v (get_slot st s))
+
+let r_child_in_store (st:vstore) (s:slot_id{store_contains st s}) : bool
+  = VStoreE?.r_child_in_store (Some?.v (get_slot st s))
+
+let has_key (k:key) (e:option vstore_entry) : bool
+  = match e with
+    | Some (VStoreE k' _ _ _ _) -> k = k'
+    | None -> false
+
+let lookup_key (st:vstore) (k:key) 
+  : option vstore_entry
+  = let s' = filter (has_key k) st in
+    if Seq.length s' = 0 then None
+    else Seq.index s' 0 
+
+let store_contains_key (st:vstore) (k:key) : bool
+  = Some? (lookup_key st k)
+
+let lemma_lookup_key_returns_k (st:vstore) (k:key) 
+  : Lemma (requires (store_contains_key st k))
+          (ensures (VStoreE?.k (Some?.v (lookup_key st k)) = k))
+  = lemma_filter_correct1 (has_key k) st 0
+
+let stored_value_by_key (st:vstore) (k:key{store_contains_key st k})
+  : value_type_of k
+  = lemma_lookup_key_returns_k st k;
+    VStoreE?.v (Some?.v (lookup_key st k))
+
+let add_method_of_by_key (st:vstore) (k:key{store_contains_key st k})
+  : add_method
+  = VStoreE?.am (Some?.v (lookup_key st k))
+
+let update_slot (st:vstore) (s:st_index st) (e:vstore_entry)
+  : vstore
+  = Seq.upd st s (Some e)
+
+let update_value
+  (st:vstore)
+  (s:slot_id{store_contains st s}) 
+  (v:value_type_of (stored_key st s))
+  : Tot (st':vstore {store_contains st' s /\
+                     stored_value st' s = v})
+  = let Some (VStoreE k _ am l r) = get_slot st s in
+    update_slot st s (VStoreE k v am l r) 
+
+let update_in_store 
+  (st:vstore)
+  (s:slot_id{store_contains st s}) 
+  (d:bin_tree_dir)
+  (b:bool)
+  : Tot (st':vstore {store_contains st' s /\
+                     (match d with
+                      | Left -> l_child_in_store st' s = b
+                      | Right -> r_child_in_store st' s = b)})
+  = let Some (VStoreE k v am l r) = get_slot st s in
+    match d with
+    | Left -> update_slot st s (VStoreE k v am b r) 
+    | Right -> update_slot st s (VStoreE k v am l b)
+
+let add_to_store 
+      (st:vstore) 
+      (s:st_index st{not (store_contains st s)}) 
+      (k:key) 
+      (v:value_type_of k)
+      (am:add_method)
+  : Tot (st':vstore {store_contains st' s /\
+                     stored_key st' s = k /\
+                     stored_value st' s = v /\
+                     add_method_of st' s = am})
+  = update_slot st s (VStoreE k v am false false)
+
+let evict_from_store
+      (st:vstore) 
+      (s:slot_id{store_contains st s})
+  : Tot (st':vstore {not (store_contains st' s)})
+  = Seq.upd st s None
