intermediate/Veritas.Intermediate.StoreS.fsti
@@ -1,0 +1,288 @@
+module Veritas.Intermediate.StoreS
+
+open Veritas.BinTree
+open Veritas.Key
+open Veritas.Record
+open Veritas.SeqAux
+
+module Spec = Veritas.Verifier
+module SC = Veritas.Intermediate.StoreSC
+
+let slot_id = nat
+let add_method = Spec.add_method
+
+type vstore_entry = 
+  | VStoreE: k:key -> 
+             v:value_type_of k -> 
+             am:add_method -> 
+             l_child_in_store:bool ->
+             r_child_in_store:bool ->
+             vstore_entry
+
+type vstore = Seq.seq (option vstore_entry) 
+
+let empty_store (n:nat) :vstore = Seq.create n None
+
+let st_index (st:vstore) = seq_index st
+
+val store_contains (st:vstore) (s:slot_id) : bool
+
+val stored_key (st:vstore) (s:slot_id{store_contains st s}) : key
+
+val stored_value (st:vstore) (s:slot_id{store_contains st s}) : value
+
+val add_method_of (st:vstore) (s:slot_id{store_contains st s}) : add_method
+
+val l_child_in_store (st:vstore) (s:slot_id{store_contains st s}) : bool
+
+val r_child_in_store (st:vstore) (s:slot_id{store_contains st s}) : bool
+
+val store_contains_key (st:vstore) (k:key) : bool
+
+val stored_value_by_key (st:vstore) (k:key{store_contains_key st k}) : value_type_of k
+
+val add_method_of_by_key (st:vstore) (k:key{store_contains_key st k}) : add_method
+
+val update_value 
+      (st:vstore) 
+      (s:slot_id{store_contains st s}) 
+      (v:value_type_of (stored_key st s))
+  : Tot (st':vstore {store_contains st' s /\ stored_value st' s = v})
+
+val update_in_store 
+  (st:vstore)
+  (s:slot_id{store_contains st s}) 
+  (d:bin_tree_dir)
+  (b:bool)
+  : Tot (st':vstore {store_contains st' s /\
+                     (match d with
+                      | Left -> l_child_in_store st' s = b
+                      | Right -> r_child_in_store st' s = b)})
+
+val add_to_store 
+      (st:vstore) 
+      (s:st_index st{not (store_contains st s)})
+      (k:key) 
+      (v:value_type_of k)
+      (am:add_method)
+  : Tot (st':vstore {store_contains st' s /\
+                     stored_key st' s = k /\
+                     stored_value st' s = v /\
+                     add_method_of st' s = am})
+
+val evict_from_store 
+      (st:vstore) 
+      (s:slot_id{store_contains st s})
+  : Tot (st':vstore {not (store_contains st' s)})
+
+(* How to check that a key is not in the store with add_method=MAdd:
+   1. If a child_in_store flag is unset then the corresponding descendent is not in the store.
+   2. k' point to the nearest descendent in the store.
+      (a) If k' points to k2 then no key between k' and k2 is in the store.
+      (b) If k' points to Empty then no descendent of k' in that direction is in the store.
+      
+   How to check that a key is not in the store with add_method=BAdd PROVIDED that the add/evict 
+   set hashes have not diverged:
+   1, If the evicted_to_blum flag is unset then the corresponding descendent is not in the store. 
+   2. Same as above. *)
+let store_contains_key_with_am (st:vstore) (k:key) (am:add_method) : bool
+  = store_contains_key st k && add_method_of_by_key st k = am
+
+let in_store_flag_unset_implies_desc_not_in_store
+      (st:vstore)
+      (s:slot_id{store_contains st s /\ MVal? (stored_value st s)})
+  = let v = to_merkle_value (stored_value st s) in    
+    let ld = desc_hash_dir v Left in
+    let rd = desc_hash_dir v Right in
+    (Desc? ld /\ not (l_child_in_store st s) ==>
+       not (store_contains_key_with_am st (Desc?.k ld) Spec.MAdd)) /\
+    (Desc? rd /\ not (r_child_in_store st s) ==> 
+       not (store_contains_key_with_am st (Desc?.k rd) Spec.MAdd))
+
+let evicted_to_blum_flag_unset_implies_desc_not_in_store
+      (st:vstore)
+      (s:slot_id{store_contains st s /\ MVal? (stored_value st s)})
+  = let v = to_merkle_value (stored_value st s) in    
+    let ld = desc_hash_dir v Left in
+    let rd = desc_hash_dir v Right in
+    (Desc? ld /\ not (Desc?.b ld) ==>
+       not (store_contains_key_with_am st (Desc?.k ld) Spec.BAdd)) /\
+    (Desc? rd /\ not (Desc?.b rd) ==> 
+       not (store_contains_key_with_am st (Desc?.k rd) Spec.BAdd))
+
+let points_to_nearest_desc_in_store 
+      (st:vstore)
+      (s:slot_id{store_contains st s /\ MVal? (stored_value st s)})
+      (am:add_method)
+  = let k' = stored_key st s in
+    let v' = to_merkle_value (stored_value st s) in
+    forall (k:key{is_proper_desc k k'}).
+    let dh = desc_hash_dir v' (desc_dir k k') in
+    if Empty? dh then not (store_contains_key_with_am st k am)
+    else if is_proper_desc (Desc?.k dh) k then not (store_contains_key_with_am st k am) 
+    else True
+
+// always true by the structure of vaddm
+let merkle_store_inv (st:vstore) = 
+  forall (s:slot_id{store_contains st s /\ MVal? (stored_value st s)}).
+    in_store_flag_unset_implies_desc_not_in_store st s /\ 
+    points_to_nearest_desc_in_store st s Spec.MAdd
+
+// only true when the add/evict set hashes have not diverged
+let blum_store_inv (st:vstore) = 
+  forall (s:slot_id{store_contains st s /\ MVal? (stored_value st s)}).
+    evicted_to_blum_flag_unset_implies_desc_not_in_store st s /\ 
+    points_to_nearest_desc_in_store st s Spec.BAdd
+
+let store_contains_st_index (st:vstore) (s:slot_id{store_contains st s})
+  : Lemma (s < Seq.length st)
+          [SMTPat (store_contains st s)] 
+  = admit()
+
+let stored_value_matches_stored_key (st:vstore) (s:slot_id{store_contains st s}) 
+  : Lemma (is_value_of (stored_key st s) (stored_value st s))
+    [SMTPat (is_value_of (stored_key st s) (stored_value st s))]
+  = admit()
+
+let update_value_preserves_length 
+      (st:vstore) 
+      (s:slot_id{store_contains st s}) 
+      (v:value_type_of (stored_key st s)) 
+  : Lemma (let st' = update_value st s v in
+           Seq.length st = Seq.length st')
+          [SMTPat (update_value st s v)]  
+  = admit()
+
+let lemma_update_value_preserves_slots
+      (st:vstore) 
+      (s:slot_id{store_contains st s}) 
+      (v:value_type_of (stored_key st s))
+      (s':st_index st)
+  : Lemma (store_contains st s' = store_contains (update_value st s v) s')
+          [SMTPat (store_contains (update_value st s v) s')]
+  = admit()
+
+let lemma_update_value_preserves_keys 
+  (st:vstore)
+  (s:slot_id{store_contains st s}) 
+  (v:value_type_of (stored_key st s))
+  (s':slot_id{store_contains st s'})
+  : Lemma (ensures stored_key st s' = stored_key (update_value st s v) s')
+          [SMTPat (stored_key (update_value st s v) s')]
+  = admit()
+
+let lemma_update_in_store_preserves_slots
+  (st:vstore)
+  (s:slot_id{store_contains st s}) 
+  (d:bin_tree_dir)
+  (b:bool)
+  (s':slot_id)
+  : Lemma (ensures store_contains st s' = store_contains (update_in_store st s d b) s')
+          [SMTPat (store_contains (update_in_store st s d b) s')]
+  = admit()
+
+let lemma_add_to_store_preserves_slots 
+      (st:vstore) 
+      (s:st_index st{not (store_contains st s)})
+      (k:key) 
+      (v:value_type_of k)
+      (am:add_method)
+      (s':slot_id{s <> s'})
+  : Lemma (ensures store_contains st s' = store_contains (add_to_store st s k v am) s')
+          [SMTPat (store_contains (add_to_store st s k v am) s')]
+  = admit()
+
+(* Relation between SC and S stores *)
+let convert_entry (eo:option vstore_entry) : option SC.vstore_entry =
+  match eo with
+  | None -> None
+  | Some e -> Some (SC.VStoreE e.k e.v e.am)
+let equal_contents (st:vstore) (st':SC.vstore) : Type
+  = Seq.equal (map convert_entry st) st'.SC.data
+
+let lemma_equal_contents_store_contains
+      (st:vstore)
+      (st':SC.vstore)
+      (s:slot_id)
+  : Lemma (requires equal_contents st st')
+          (ensures store_contains st s = SC.store_contains st' s)
+          [SMTPat (store_contains st s); SMTPat (SC.store_contains st' s)]
+  = admit()
+
+let lemma_equal_contents_store_contains_key
+      (st:vstore)
+      (st':SC.vstore)
+      (k:key)
+  : Lemma (requires equal_contents st st')
+          (ensures store_contains_key st k = SC.store_contains_key st' k)
+          [SMTPat (store_contains_key st k); SMTPat (SC.store_contains_key st' k)]
+  = admit()
+
+let lemma_equal_contents_stored_key
+      (st:vstore)
+      (st':SC.vstore)
+      (s:slot_id{store_contains st s})
+  : Lemma (requires equal_contents st st')
+          (ensures stored_key st s = SC.stored_key st' s)
+          [SMTPat (stored_key st s); SMTPat (SC.stored_key st' s)]
+  = admit()
+
+let lemma_equal_contents_stored_value
+      (st:vstore)
+      (st':SC.vstore)
+      (s:slot_id{store_contains st s})
+  : Lemma (requires equal_contents st st')
+          (ensures stored_value st s = SC.stored_value st' s)
+          [SMTPat (stored_value st s); SMTPat (SC.stored_value st' s)]
+  = admit()
+
+let lemma_equal_contents_add_method_of
+      (st:vstore)
+      (st':SC.vstore)
+      (s:slot_id{store_contains st s})
+  : Lemma (requires equal_contents st st')
+          (ensures add_method_of st s = SC.add_method_of st' s)
+          [SMTPat (add_method_of st s); SMTPat (SC.add_method_of st' s)]
+  = admit()
+
+let lemma_equal_contents_update_value
+  (st:vstore)
+  (st':SC.vstore)
+  (s:slot_id{store_contains st s}) 
+  (v:value_type_of (stored_key st s))
+  : Lemma (requires equal_contents st st')
+          (ensures equal_contents (update_value st s v) (SC.update_store st' s v))
+          [SMTPat (equal_contents (update_value st s v) (SC.update_store st' s v))]
+  = admit()
+
+let lemma_equal_contents_update_in_store
+  (st:vstore)
+  (st':SC.vstore)
+  (s:slot_id{store_contains st s}) 
+  (d:bin_tree_dir)
+  (b:bool)
+  : Lemma (requires equal_contents st st')
+          (ensures equal_contents (update_in_store st s d b) st')
+          [SMTPat (equal_contents (update_in_store st s d b) st')]
+  = admit()
+
+let lemma_equal_contents_add_to_store 
+      (st:vstore) 
+      (st':SC.vstore)
+      (s:st_index st{not (store_contains st s)})
+      (k:key) 
+      (v:value_type_of k)
+      (am:add_method)
+  : Lemma (requires equal_contents st st')
+          (ensures equal_contents (add_to_store st s k v am) (SC.add_to_store st' s k v am))
+          [SMTPat (equal_contents (add_to_store st s k v am) (SC.add_to_store st' s k v am))]
+  = admit()
+
+let lemma_equal_contents_evict_from_store
+      (st:vstore) 
+      (st':SC.vstore)
+      (s:st_index st{store_contains st s})
+  : Lemma (requires equal_contents st st')
+          (ensures equal_contents (evict_from_store st s) (SC.evict_from_store st' s))
+          [SMTPat (equal_contents (evict_from_store st s) (SC.evict_from_store st' s))]
+  = admit()
