intermediate/Veritas.Intermediate.VerifyS.fst
@@ -1,0 +1,3 @@
+module Veritas.Intermediate.VerifyS
+
+// Everything is in the fsti file for now. Will move later.
