intermediate/Veritas.Intermediate.VerifyS.fsti
@@ -1,0 +1,567 @@
+module Veritas.Intermediate.VerifyS
+
+open Veritas.Intermediate.Logs
+open Veritas.Intermediate.StoreS
+
+open Veritas.BinTree
+open Veritas.Hash
+open Veritas.Key
+open Veritas.MultiSetHash
+open Veritas.MultiSetHashDomain
+open Veritas.Record
+open Veritas.SeqAux
+
+module Spec = Veritas.Verifier
+module SC = Veritas.Intermediate.VerifySC
+module SCstore = Veritas.Intermediate.StoreSC
+
+(* Thread-local state
+   id     : thread id
+   st     : thread local store
+   clock  : current timestamp
+   hadd   : add set hash
+   hevict : evict set hash *)
+noeq
+type vtls =
+  | Failed : vtls
+  | Valid :
+    id : thread_id ->
+    st : vstore ->
+    clock : timestamp ->
+    hadd : ms_hash_value -> // TODO: should be a multiset
+    hevict : ms_hash_value -> // TODO: should be a (multi?)set
+    vtls
+
+let thread_id_of (vs:vtls {Valid? vs}): thread_id = 
+  Valid?.id vs
+
+let thread_store (vs: vtls {Valid? vs}): vstore =
+  Valid?.st vs
+
+let thread_store_size (vs: vtls {Valid? vs}): nat =
+  let st = thread_store vs in Seq.length st
+
+let update_thread_store (vs:vtls {Valid? vs}) (st:vstore) : vtls =
+  match vs with
+  | Valid id _ clock hadd hevict -> Valid id st clock hadd hevict
+
+let thread_clock (vs:vtls {Valid? vs}) = 
+  Valid?.clock vs
+
+let update_thread_clock (vs:vtls {Valid? vs}) (clock:timestamp): vtls = 
+  match vs with
+  | Valid id st _ hadd hevict -> Valid id st clock hadd hevict
+
+let thread_hadd (vs:vtls {Valid? vs}) = 
+  Valid?.hadd vs
+
+let thread_hevict (vs:vtls {Valid? vs}) = 
+  Valid?.hevict vs
+
+let update_thread_hadd (vs:vtls {Valid? vs}) (hadd: ms_hash_value): vtls = 
+  match vs with
+  | Valid id st clock _ hevict -> Valid id st clock hadd hevict
+
+let update_thread_hevict (vs:vtls {Valid? vs}) (hevict:ms_hash_value): vtls = 
+  match vs with
+  | Valid id st clock hadd _ -> Valid id st clock hadd hevict
+
+let vget (s:slot_id) (k:key) (v:data_value) (vs: vtls {Valid? vs}) : vtls =
+  let st = thread_store vs in
+  (* check store contains slot s *)
+  if not (store_contains st s) then Failed
+  (* check stored key and value *)
+  else let k' = stored_key st s in
+       let v' = stored_value st s in
+       if k <> k' then Failed
+       else if not (DVal? v') then Failed
+       else if to_data_value v' <> v then Failed
+       else vs
+
+let vput (s:slot_id) (k:key) (v:data_value) (vs: vtls {Valid? vs}) : vtls =
+  let st = thread_store vs in
+  (* check store contains slot s *)
+  if not (store_contains st s) then Failed
+  (* check stored key is k *)
+  else let k' = stored_key st s in
+       if k <> k' then Failed
+       else if not (is_data_key (stored_key st s)) then Failed
+       else update_thread_store vs (update_value st s (DVal v))
+
+let vaddm (s:slot_id) (r:record) (s':slot_id) (vs: vtls {Valid? vs}): vtls =
+  if not (s < thread_store_size vs) then Failed
+  else 
+    let st = thread_store vs in
+    let (k,v) = r in
+    (* check store contains slot s' *)
+    if not (store_contains st s') then Failed
+    else
+      let k' = stored_key st s' in
+      let v' = stored_value st s' in
+      (* check k is a proper desc of k' *)
+      if not (is_proper_desc k k') then Failed
+      (* check store does not contain slot s *)
+      else if store_contains st s then Failed
+      (* check type of v is consistent with k *)
+      else if not (is_value_of k v) then Failed
+      (* check v' is a merkle value *)
+      else if DVal? v' then Failed 
+      else
+        let v' = to_merkle_value v' in
+        let d = desc_dir k k' in
+        let dh' = desc_hash_dir v' d in 
+        let h = hashfn v in
+        match dh' with
+        | Empty -> (* k' has no child in direction d *)
+            (* first add must be init value *)
+            if v <> init_value k then Failed
+            else
+              let v'_upd = Spec.update_merkle_value v' d k h false in
+              let st_upd = update_value st s' (MVal v'_upd) in
+              let st_upd2 = add_to_store st_upd s k v Spec.MAdd in
+              let st_upd3 = update_in_store st_upd2 s' d true in
+              update_thread_store vs st_upd3
+        | Desc k2 h2 b2 -> 
+            if k2 = k 
+            then (* k is a child of k' *)
+              (* check hashes match and k was not evicted to blum *)
+              if not (h2 = h && b2 = false) then Failed
+              (* check store does not contain k*)
+              else if Left? d && l_child_in_store st s' then Failed
+              else if Right? d && r_child_in_store st s' then Failed
+              else 
+                let st_upd = add_to_store st s k v Spec.MAdd in
+                let st_upd2 = update_in_store st_upd s' d true in
+                update_thread_store vs st_upd2
+            else (* otherwise, k is not a child of k' *)
+            (* first add must be init value *)
+            if v <> init_value k then Failed
+            (* check k2 is a proper desc of k *)
+            else if not (is_proper_desc k2 k) then Failed
+            else
+              let d2 = desc_dir k2 k in
+              let mv = to_merkle_value v in
+              let mv_upd = Spec.update_merkle_value mv d2 k2 h2 b2 in
+              let v'_upd = Spec.update_merkle_value v' d k h false in
+              let st_upd = update_value st s' (MVal v'_upd) in
+              let st_upd2 = add_to_store st_upd s k (MVal mv_upd) Spec.MAdd in
+              let st_upd3 = update_in_store st_upd2 s' d true in
+              let st_upd4 = update_in_store st_upd3 s d2 true in
+              update_thread_store vs st_upd4
+
+let has_instore_merkle_desc (st:vstore) (s:slot_id{store_contains st s}): bool = 
+  let k = stored_key st s in
+  if is_data_key k then false
+  else 
+    // TODO: remove the assert with a better SMTPat for stored_value_matches_stored_key
+    let _ = assert (is_value_of k (stored_value st s)) in   
+    let v = to_merkle_value (stored_value st s) in
+    let ld = desc_hash_dir v Left in
+    let rd = desc_hash_dir v Right in
+    Desc? ld && l_child_in_store st s || 
+    Desc? rd && r_child_in_store st s
+
+let vevictm (s:slot_id) (s':slot_id) (vs: vtls {Valid? vs}): vtls = 
+  let st = thread_store vs in
+  (* check store contains s and s' *)
+  if not (store_contains st s && store_contains st s') then Failed
+  else 
+    let k = stored_key st s in
+    let v = stored_value st s in
+    let k' = stored_key st s' in
+    let v' = stored_value st s' in
+    (* check k is a proper descendent of k' *)
+    if not (is_proper_desc k k') then Failed
+    (* check k does not have a child in the store *)
+    else if has_instore_merkle_desc st s then Failed
+    else
+      let d = desc_dir k k' in
+      // TODO: remove the assert with a better SMTPat for stored_value_matches_stored_key
+      let _ = assert (is_value_of k' v') in 
+      let v' = to_merkle_value v' in
+      let dh' = desc_hash_dir v' d in
+      let h = hashfn v in
+      match dh' with
+      | Empty -> Failed
+      | Desc k2 h2 b2 -> 
+          if k2 <> k then Failed
+          else
+            let v'_upd = Spec.update_merkle_value v' d k h false in
+            let st_upd = update_value st s' (MVal v'_upd) in
+            let st_upd2 = evict_from_store st_upd s in
+            update_thread_store vs st_upd2
+
+let vaddb (s:slot_id) (r:record) (t:timestamp) (j:thread_id) (vs:vtls {Valid? vs}): vtls = 
+  if not (s < thread_store_size vs) then Failed
+  else
+    let st = thread_store vs in 
+    let (k,v) = r in
+    (* check value type consistent with key k *)
+    if not (is_value_of k v) then Failed
+    (* check store contains slot s *)
+    else if store_contains st s then Failed
+    else 
+      (* update add hash *)
+      let h = thread_hadd vs in
+      let h_upd = ms_hashfn_upd (MHDom (k,v) t j) h in
+      let vs_upd = update_thread_hadd vs h_upd in
+      (* update clock *)
+      let clk = thread_clock vs in
+      let clk_upd = Spec.max clk (next t) in
+      let vs_upd2 = update_thread_clock vs_upd clk_upd in
+      (* add record to store *)
+      let st_upd = add_to_store st s k v Spec.BAdd in
+      update_thread_store vs_upd2 st_upd
+
+let vevictb (s:slot_id) (t:timestamp) (vs:vtls {Valid? vs}): vtls = 
+  let clock = thread_clock vs in
+  let st = thread_store vs in
+  (* check store contains slot s *)
+  if not (store_contains st s) then Failed
+  else
+    let k = stored_key st s in
+    let v = stored_value st s in
+    (* check key at s is not root *)
+    if k = Root then Failed
+    (* check time of evict < current time *)
+    else if not (ts_lt clock t) then Failed
+    (* check s was added through blum *)  
+    else if add_method_of st s <> Spec.BAdd then Failed
+    (* check k has no children n the store *)
+    else if has_instore_merkle_desc st s then Failed  
+    else 
+      (* update evict hash *)
+      let h = thread_hevict vs in
+      let h_upd = ms_hashfn_upd (MHDom (k,v) t (thread_id_of vs)) h in
+      let vs_upd = update_thread_hevict vs h_upd in
+      (* update clock *)
+      let vs_upd2 = update_thread_clock vs_upd t in    
+      (* evict record *)
+      let st_upd = evict_from_store st s in
+      update_thread_store vs_upd2 st_upd
+
+let vevictbm (s:slot_id) (s':slot_id) (t:timestamp) (vs:vtls {Valid? vs}): vtls = 
+  let st = thread_store vs in
+  (* check store contains s and s' *)
+  if not (store_contains st s && store_contains st s') then Failed
+  else
+    let k = stored_key st s in
+    let k' = stored_key st s' in
+    let v' = stored_value st s' in
+    (* check k is a proper desc of k' *)
+    if not (is_proper_desc k k') then Failed
+    (* check s was added through merkle *)
+    else if add_method_of st s <> Spec.MAdd then Failed  
+    (* check k has no children in the store *)
+    else if has_instore_merkle_desc st s then Failed  
+    else
+      // TODO: remove the assert with a better SMTPat for stored_value_matches_stored_key
+      let _ = assert (is_value_of k' v') in 
+      let v' = to_merkle_value v' in
+      let d = desc_dir k k' in
+      let dh' = desc_hash_dir v' d in
+      match dh' with
+      | Empty -> Failed
+      | Desc k2 h2 b2 -> 
+          if k2 <> k || b2 then Failed
+          else
+            let v'_upd = Spec.update_merkle_value v' d k h2 true in
+            let st_upd = update_value st s' (MVal v'_upd) in
+            vevictb s t (update_thread_store vs st_upd)
+
+(* Relation between SC and S thread-local states *)
+
+let hashes_diverged (hadd:ms_hash_value) (hevict:ms_hash_value) : bool = 
+  // TODO: informally, there is no way to extend the add or evict sets so that their hashes match
+  admit()
+  
+let vtls_rel (vs:vtls) (vs':SC.vtls) : Type =
+  (Failed? vs /\ SC.Failed? vs') \/
+  (Valid? vs /\ SC.Valid? vs' /\
+   (let (Valid id st clk ha he) = vs in
+    let (SC.Valid id' st' clk' ha' he') = vs' in
+    // all fields are equal
+    equal_contents st st' /\ id = id' /\ clk = clk' /\ ha = ha' /\ he = he' /\
+    // SC's is_map field indicates that the add/evict sets have diverged -- not needed?
+    (not (SC.thread_store_is_map vs') ==> hashes_diverged ha he) /\
+    // the invariant over MAdd keys always holds
+    merkle_store_inv st /\ 
+    // the invariant over BAdd keys holds if the add/evict sets have not diverged
+    (not (hashes_diverged ha he) ==> blum_store_inv st)))
+
+let lemma_vget_simulates_SC 
+      (vs:vtls{Valid? vs})
+      (vs':SC.vtls{SC.Valid? vs'})
+      (s:slot_id)
+      (k:data_key)
+      (v:data_value)
+  : Lemma (requires (vtls_rel vs vs'))
+          (ensures (vtls_rel (vget s k v vs) (SC.vget s k v vs')))
+          // TODO: add a condition to each 'ensures' that says that the add/evict hashes stay diverged
+  = ()
+
+let lemma_update_value_DVal_preserves_merkle_inv (st:vstore) (s:slot_id{store_contains st s /\ is_data_key (stored_key st s)}) (v:data_value)
+  : Lemma (requires merkle_store_inv st)
+          (ensures merkle_store_inv (update_value st s (DVal v)))
+          [SMTPat (merkle_store_inv (update_value st s (DVal v)))]
+  = admit()
+
+let lemma_update_value_DVal_preserves_blum_inv (st:vstore) (s:slot_id{store_contains st s /\ is_data_key (stored_key st s)}) (v:data_value)
+  : Lemma (requires blum_store_inv st)
+          (ensures blum_store_inv (update_value st s (DVal v)))
+          [SMTPat (blum_store_inv (update_value st s (DVal v)))]
+  = admit()
+
+let lemma_vput_simulates_SC
+      (vs:vtls{Valid? vs}) 
+      (vs':SC.vtls{SC.Valid? vs'}) 
+      (s:slot_id) 
+      (k:data_key) 
+      (v:data_value) 
+  : Lemma (requires (vtls_rel vs vs'))
+          (ensures (vtls_rel (vput s k v vs) (SC.vput s k v vs'))) 
+  = ()
+
+let lemma_vaddm_simulates_SC 
+      (vs:vtls{Valid? vs}) 
+      (vs':SC.vtls{SC.Valid? vs'}) 
+      (s s':slot_id)
+      (r:record)  
+  : Lemma (requires (vtls_rel vs vs'))
+          (ensures (vtls_rel (vaddm s r s' vs) (SC.vaddm s r s' vs'))) 
+  = if s < thread_store_size vs
+    then 
+      let st = thread_store vs in
+      let (k,v) = r in
+      if store_contains st s'
+      then
+        let k' = stored_key st s' in
+        let v' = stored_value st s' in
+        if is_proper_desc k k' && not (store_contains st s) && not (DVal? v')
+        then
+          let v' = to_merkle_value v' in
+          let d = desc_dir k k' in
+          let dh' = desc_hash_dir v' d in 
+          let h = hashfn v in
+          let st' = SC.thread_store vs' in
+          match dh' with
+          | Empty -> 
+              // CASE 1 - by points_to_nearest_desc_in_store, either k is not in the store or the evict/add sets have diverged
+              if v = init_value k 
+              then (
+                let v'_upd = Spec.update_merkle_value v' d k h false in
+                let st_upd = update_value st s' (MVal v'_upd) in
+                let st_upd2 = add_to_store st_upd s k v Spec.MAdd in
+                let st_upd3 = update_in_store st_upd2 s' d true in
+                assume (merkle_store_inv st_upd3);
+                if (hashes_diverged (thread_hadd vs) (thread_hevict vs))
+                then (
+                  let Valid _ st _ _ _ = update_thread_store vs st_upd3 in
+                  assume (SC.Valid? (SC.vaddm s r s' vs'));
+                  assume (not (SC.thread_store_is_map (SC.vaddm s r s' vs'))) 
+                  )
+                else (
+                  assert (points_to_nearest_desc_in_store st s' Spec.BAdd);
+                  assert (not (store_contains_key_with_am st k Spec.BAdd));
+                  assert (not (store_contains_key_with_am st k Spec.MAdd));
+                  assert (not (store_contains_key st k));
+                  lemma_equal_contents_store_contains_key st st' k;
+                  //assert (not (SCstore.store_contains_key st' k));
+                  let Valid id st clk ha he = update_thread_store vs st_upd3 in
+                  let SC.Valid id' st' clk' ha' he' = SC.vaddm s r s' vs' in
+                  assume (blum_store_inv st); // easy since we are not adding anything via BAdd
+                  admit()
+                )
+              )
+          | Desc k2 h2 b2 -> 
+              if k2 = k 
+              // CASE 2 - by in_store_flag_implies... and evicted_to_blum_flag_implies..., either k is not in the store or the evict/add sets have diverged
+              then admit()
+              // CASE 3 - similar to CASE 1
+              else admit()
+
+let lemma_evict_from_store_preserves_merkle_inv (st:vstore) (s:slot_id{store_contains st s})
+  : Lemma (requires merkle_store_inv st)
+          (ensures merkle_store_inv (evict_from_store st s))
+          [SMTPat (merkle_store_inv (evict_from_store st s))]
+  = admit()
+
+let lemma_update_evict_from_store_preserves_blum_inv (st:vstore) (s:slot_id{store_contains st s})
+  : Lemma (requires blum_store_inv st)
+          (ensures blum_store_inv (evict_from_store st s))
+          [SMTPat (blum_store_inv (evict_from_store st s))]
+  = admit()
+
+let lemma_has_in_store_merkle_desc (st:vstore) (st':SCstore.vstore) (s:slot_id{store_contains st s})
+  : Lemma (requires equal_contents st st' /\ merkle_store_inv st)
+          (ensures has_instore_merkle_desc st s = SC.has_instore_merkle_desc st' (SCstore.stored_key st' s))
+          [SMTPat (has_instore_merkle_desc st s); SMTPat (SC.has_instore_merkle_desc st' (SCstore.stored_key st' s))]
+  = admit()
+
+let lemma_vevictm_simulates_SC 
+      (vs:vtls{Valid? vs}) 
+      (vs':SC.vtls{SC.Valid? vs'}) 
+      (s s':slot_id)  
+  : Lemma (requires (vtls_rel vs vs'))
+          (ensures (vtls_rel (vevictm s s' vs) (SC.vevictm s s' vs'))) 
+  = let st = thread_store vs in
+    let st' = SC.thread_store vs' in
+    if store_contains st s && store_contains st s'
+    then 
+      let k = stored_key st s in
+      let v = stored_value st s in
+      let k' = stored_key st s' in
+      let v' = stored_value st s' in
+      if is_proper_desc k k' && not (has_instore_merkle_desc st s) 
+      then
+        let d = desc_dir k k' in
+        let _ = assert (is_value_of k' v') in 
+        let v' = to_merkle_value v' in
+        let dh' = desc_hash_dir v' d in
+        let h = hashfn v in
+        match dh' with
+        | Empty -> ()
+        | Desc k2 h2 b2 ->
+            if k2 = k
+            then
+              let v'_upd = Spec.update_merkle_value v' d k h false in
+              let st_upd = update_value st s' (MVal v'_upd) in
+              let st_upd2 = evict_from_store st_upd s in
+              let Valid id st clk ha he = update_thread_store vs st_upd2 in
+              assume (merkle_store_inv st_upd);
+              if not (hashes_diverged ha he) 
+              then assume (blum_store_inv st_upd)
+
+let lemma_vaddb_simulates_SC 
+      (vs:vtls{Valid? vs}) 
+      (vs':SC.vtls{SC.Valid? vs'}) 
+      (s:slot_id)
+      (r:record)
+      (t:timestamp)
+      (j:thread_id)
+  : Lemma (requires (vtls_rel vs vs'))
+          (ensures (vtls_rel (vaddb s r t j vs) (SC.vaddb s r t j vs')))
+  = if s < thread_store_size vs
+    then
+      let st = thread_store vs in 
+      let (k,v) = r in
+      if is_value_of k v
+      then if not (store_contains st s)
+      then
+        let h = thread_hadd vs in
+        let h_upd = ms_hashfn_upd (MHDom (k,v) t j) h in
+        let vs_upd = update_thread_hadd vs h_upd in
+        let clk = thread_clock vs in
+        let clk_upd = Spec.max clk (next t) in
+        let vs_upd2 = update_thread_clock vs_upd clk_upd in
+        let st_upd = add_to_store st s k v Spec.BAdd in
+        let Valid _ st _ ha he = update_thread_store vs_upd2 st_upd in
+        assume (merkle_store_inv st); // easy since we are not adding anything via MAdd
+        assume (not (SC.thread_store_is_map (SC.vaddb s r t j vs')) ==> hashes_diverged ha he);  
+        assume (not (hashes_diverged ha he) ==> blum_store_inv st)
+
+(* Thoughts on filling in the last two assumes:
+
+   if store_contains_key k
+   then (
+     the SC is_map flag will be false
+     hashes_diverged should be true
+     -> blum_store_inv st does not need to hold
+   )
+   else (
+     SC will leave the is_map flag unchanged
+     if blum_store_inv is violated by adding k
+     then (
+       there exists a slot s s.t.
+       (a) k is marked as a descendent of s and the evicted_to_blum flag of s is not set 
+       or (b) k is a descendent of s, but is not stored in the hash of s
+
+       ... in either case, the hashes have diverged
+     )
+     -> this proves (not hashes_diverged ==> blum_store_inv holds)
+   )
+*)
+
+let lemma_vevictb_simulates_SC 
+      (vs:vtls{Valid? vs}) 
+      (vs':SC.vtls{SC.Valid? vs'}) 
+      (s:slot_id)
+      (t:timestamp)
+  : Lemma (requires (vtls_rel vs vs'))
+          (ensures (vtls_rel (vevictb s t vs) (SC.vevictb s t vs'))) 
+  = let clock = thread_clock vs in
+    let st = thread_store vs in
+    if store_contains st s 
+    then
+      let k = stored_key st s in
+      let v = stored_value st s in
+      if k <> Root && ts_lt clock t && add_method_of st s = Spec.BAdd && not (has_instore_merkle_desc st s)
+      then
+        let h = thread_hevict vs in
+        let h_upd = ms_hashfn_upd (MHDom (k,v) t (thread_id_of vs)) h in
+        let vs_upd = update_thread_hevict vs h_upd in
+        let vs_upd2 = update_thread_clock vs_upd t in    
+        let st_upd = evict_from_store st s in
+        let Valid _ _ _ ha he = update_thread_store vs_upd2 st_upd in
+        if (hashes_diverged ha he) then assume (blum_store_inv st)
+
+let lemma_vevictbm_simulates_SC 
+      (vs:vtls{Valid? vs}) 
+      (vs':SC.vtls{SC.Valid? vs'}) 
+      (s s':slot_id)
+      (t:timestamp)
+  : Lemma (requires (vtls_rel vs vs'))
+          (ensures (vtls_rel (vevictbm s s' t vs) (SC.vevictbm s s' t vs'))) 
+  = let st = thread_store vs in
+    if store_contains st s && store_contains st s' 
+    then
+      let k = stored_key st s in
+      let k' = stored_key st s' in
+      let v' = stored_value st s' in
+      if is_proper_desc k k' && add_method_of st s = Spec.MAdd && not (has_instore_merkle_desc st s)
+      then
+        let _ = assert (is_value_of k' v') in 
+        let v' = to_merkle_value v' in
+        let d = desc_dir k k' in
+        let dh' = desc_hash_dir v' d in
+        match dh' with
+        | Empty -> ()
+        | Desc k2 h2 b2 -> 
+            if k2 = k && not b2 
+            then (
+              let v'_upd = Spec.update_merkle_value v' d k h2 true in
+              let st_upd = update_value st s' (MVal v'_upd) in
+              let st' = SC.thread_store vs' in
+              let st_upd' = SCstore.update_store st' s' (MVal v'_upd) in
+              let Valid id st clk ha he = update_thread_store vs st_upd in
+              assume (merkle_store_inv st_upd); // same assumes as vevictm
+              if not (hashes_diverged ha he) 
+              then assume (blum_store_inv st_upd);
+              lemma_vevictb_simulates_SC (update_thread_store vs st_upd) (SC.update_thread_store vs' st_upd') s t
+            )
+
+let t_verify_step (vs:vtls) (e:logS_entry): vtls =
+  match vs with
+  | Failed -> Failed
+  | _ ->
+    match e with
+    | Get_S s k v -> vget s k v vs
+    | Put_S s k v -> vput s k v vs
+    | AddM_S s r s' -> vaddm s r s' vs
+    | EvictM_S s s' -> vevictm s s' vs
+    | AddB_S s r t j -> vaddb s r t j vs
+    | EvictB_S s t -> vevictb s t vs
+    | EvictBM_S s s' t -> vevictbm s s' t vs
+
+(* Verify a log from a specified initial state *)
+let rec t_verify_aux (vs:vtls) (l:logS): Tot vtls
+  (decreases (Seq.length l)) =
+  let n = Seq.length l in
+  if n = 0 then vs
+  else
+    let lp = prefix l (n - 1) in
+    let vsp = t_verify_aux vs lp in
+    let e = Seq.index l (n - 1) in
+    t_verify_step vsp e
+
+// ... 
